\begin{proof}
  We proceed by induction on $n$.  In the base case of $n = 1$, the
  result is immediate from
  Lemma~\ref{lem:lvars-strong-one-sided-confluence}.

  For the induction step, suppose $\conf \parstepsto^n \conf'
  \parstepsto \conf'''$ and suppose the lemma holds for $n$.

  We show that it holds for $n + 1$, as follows.

  We are required to show that there exist $\conf_c, i, j$ such that
  $\conf''' \parstepsto^i \conf_c$ and $\conf'' \parstepsto^j \conf_c$
  and $i \leq m$ and $j \leq n + 1$.

  From the induction hypothesis, we have that there exist $\conf'_c,
  i', j'$ such that $\conf' \parstepsto^{i'} \conf'_c$ and $\conf''
  \parstepsto^{j'} \conf'_c$ and $i' \leq m$ and $j' \leq n$.

  We proceed by cases on $i'$:
  \begin{itemize}

  \item If $i' = 0$, then $\conf' = \conf_c'$.  We can then choose
    $\conf_c = \conf'''$ and $i = 0$ and $j = j' + 1$.

  \item If $i' \geq 1$:

    From $\conf' \parstepsto \conf'''$ and $\conf' \parstepsto^{i'}
    \conf_c'$ and Lemma~\ref{lem:lvars-strong-one-sided-confluence},
    we have that there exist $\conf_c''$ and $i''$ and $j''$ such that
    $\conf''' \parstepsto^{i''} \conf_c''$ and $\conf_c'
    \parstepsto^{j''} \conf_c''$ and $i'' \leq i'$ and $j'' \leq 1$.
    So we also have $\conf'' \parstepsto^{j'} \conf_c'
    \parstepsto^{j''} \conf_c''$.  In summary, we pick $\conf_c =
    \conf_c''$ and $i = i''$ and $j = j' + j''$, which is sufficient
    because $i = i'' \leq i' \leq m$ and $j = j' + j'' \leq n + 1$.
  \end{itemize}

\end{proof}
