\begin{proof}
  Consider arbitrary $S''$ such that $S''$ is non-conflicting with
  $\config{S}{e} \parstepsto \config{S'}{e'}$ and $\lubstore{S'}{S''}
  = \topS$.

  To show: There exists $i \leq 1$ such that
  $\config{\lubstore{S}{S''}}{e} \parstepsto^i \error$.

  The proof is by cases on the rule of the reduction semantics by
  which $\config{S}{e}$ steps to $\config{S'}{e'}$.  Since
  $\config{S'}{e'} \neq \error$, we do not need to consider the {\sc
    E-Put-Err} rule.
  \begin{itemize}

    \item Case {\sc E-Beta}:

      Given: $\config{S}{\app{(\lam{x}{e})}{v}} \parstepsto
      \config{S}{\subst{e}{x}{v}}$.

      To show: $\config{\lubstore{S}{S''}}{\app{(\lam{x}{e})}{v}}
      \parstepsto^i \error$, where $i \leq 1$.

      By assumption, $\lubstore{S}{S''} = \topS$.

      Hence, by the definition of $\error$,
      $\config{\lubstore{S}{S''}}{\app{(\lam{x}{e})}{v}} = \error$.

      Hence $\config{\lubstore{S}{S''}}{\app{(\lam{x}{e})}{v}}
      \parstepsto^i \error$, with $i = 0$.

    \item Case {\sc E-New}:

      Given: $\config{S}{\NEW} \parstepsto
      \config{\extSRaw{S}{l}{\bot}}{l}$.

      To show: $\config{\lubstore{S}{S''}}{\NEW} \parstepsto^i
      \error$, where $i \leq 1$.

      By {\sc E-New}, $\config{\lubstore{S}{S''}}{\NEW} \parstepsto
      \config{\extSRaw{(\lubstore{S}{S''})}{l'}{\bot}}{l'}$, where $l'
      \notin \dom{\lubstore{S}{S''}}$.

      By assumption, $S''$ is non-conflicting with $\config{S}{\NEW}
      \parstepsto \config{\extSRaw{S}{l}{\bot}}{l}$.
 
      Therefore $l \notin \dom{S''}$.

      From the side condition of {\sc E-New}, $l \notin \dom{S}$.

      Therefore $l \notin \dom{\lubstore{S}{S''}}$.

      Therefore, in
      $\config{\extSRaw{(\lubstore{S}{S''})}{l'}{\bot}}{l'}$, we can
      $\alpha$-rename $l'$ to $l$, \\ resulting in
      $\config{\extSRaw{(\lubstore{S}{S''})}{l}{\bot}}{l}$.

      Therefore $\config{\lubstore{S}{S''}}{\NEW} \parstepsto
      \config{\extSRaw{(\lubstore{S}{S''})}{l}{\bot}}{l}$.

      By assumption, $\lubstore{\extSRaw{S}{l}{\bot}}{S''}
      = \topS$.

      Note that:
      \begin{align*}
        \topS &= \lubstore{\extSRaw{S}{l}{\bot}}{S''} \\ &=
        \lubstore{\lubstore{S}{\store{\storebindingRaw{l}{\bot}}}}{S''}
        \\ &=
        \lubstore{\lubstore{S}{S''}}{\store{\storebindingRaw{l}{\bot}}}
        \\ &=
        \lubstore{(\lubstore{S}{S''})}{\store{\storebindingRaw{l}{\bot}}}
        \\ &= \extSRaw{(\lubstore{S}{S''})}{l}{\bot} .
      \end{align*}

      Hence $\config{\lubstore{S}{S''}}{\NEW} \parstepsto
      \config{\topS}{l}$.

      Hence, by the definition of $\error$,
      $\config{\lubstore{S}{S''}}{\NEW} \parstepsto \error$.

      Hence $\config{\lubstore{S}{S''}}{\NEW} \parstepsto^i \error$,
      with $i = 1$.

    \item Case {\sc E-Put}:

      Given: $\config{S}{\putexp{l}{d_2}} \parstepsto
      \config{\extSRaw{S}{l}{d_2}}{\unit}$.

      To show: $\config{\lubstore{S}{S''}}{\putexp{l}{d_2}}
      \parstepsto^i \error$, where $i \leq 1$.

      We proceed by cases on $\lubstore{S}{S''}$:

      \begin{itemize}

        \item $\lubstore{S}{S''} = \topS$:

          In this case, by the definition of $\error$,
          $\config{\lubstore{S}{S''}}{\putexp{l}{d_2}} = \error$.

          Hence $\config{\lubstore{S}{S''}}{\putexp{l}{d_2}}
          \parstepsto^i \error$, with $i = 0$.

        \item $\lubstore{S}{S''} \neq \topS$:

          From the premises of {\sc E-Put}, we have that $S(l) = d_1$.

          Hence $(\lubstore{S}{S''})(l) = d'_1$, where $d_1 \userleq
          d'_1$.

          We show that $\userlub{d'_1}{d_2} =
          \top$, as follows:

          By assumption, $\lubstore{\extSRaw{S}{l}{d_2}}{S''} = \topS$.

          Hence, by Definition~\ref{def:lvars-lubstore}, there exists
          some $l' \in \dom{\extSRaw{S}{l}{d_2}} \cap \dom{S''}$ such
          that $\userlub{(\extSRaw{S}{l}{d_2})(l')}{S''(l')} = \top$.

          Now case on $l'$:

          \begin{itemize}
            \item $l' \neq l$:

              In this case, $(\extSRaw{S}{l}{d_2})(l') = S(l')$.

              Since $\userlub{(\extSRaw{S}{l}{d_2})(l')}{S''(l')} = \top$,
              we then have that $\userlub{S(l')}{S''(l')} = \top$.

              However, this is a contradiction since
              $\lubstore{S}{S''} \neq \topS$.

              Hence this case cannot occur.

            \item $l' = l$:

              Then $\userlub{(\extSRaw{S}{l}{d_2})(l)}{S''(l)} = \top$.

              Note that:
              \begin{align*}
                \top &= \userlub{(\extSRaw{S}{l}{d_2})(l)}{S''(l)} \\ &=
                \userlub{d_2}{S''(l)} \\ &=
                \userlub{\userlub{d_1}{d_2}}{S''(l)}
                \\ &=
                \userlub{\userlub{S(l)}{d_2}}{S''(l)}
                \\ &=
                \userlub{\userlub{S(l)}{S''(l)}}{d_2}
                \\ &=
                \userlub{(\lubstore{S}{S''})(l)}{d_2}
                \\ &= \userlub{d'_1}{d_2}.
              \end{align*}
              Hence $\userlub{d'_1}{d_2} = \top$.

              Hence, by {\sc E-Put-Err},
              $\config{\lubstore{S}{S''}}{\putexp{l}{d_2}} \parstepsto
              \error$.

              Hence $\config{\lubstore{S}{S''}}{\putexp{l}{d_2}}
              \parstepsto^i \error$, with $i = 1$.

          \end{itemize}

      \end{itemize}

    \item Case {\sc E-Get}:

      Given: $\config{S}{\getexp{l}{T}} \parstepsto \config{S}{d_2}$.

      To show: $\config{\lubstore{S}{S''}}{\getexp{l}{T}}
      \parstepsto^i \error$, where $i \leq 1$.

      By assumption, $\lubstore{S}{S''} = \topS$.

      Hence, by the definition of $\error$,
      $\config{\lubstore{S}{S''}}{\getexp{l}{T}} = \error$.

      Hence $\config{\lubstore{S}{S''}}{\getexp{l}{T}} \parstepsto^i
      \error$, with $i = 0$.
  \end{itemize}
\end{proof}
