\begin{proof}
  We proceed by induction on $m$.  In the base case of $m = 1$, the
  result is immediate from
  Lemma~\ref{lem:strong-local-quasi-confluence}, with $k = 1$.

  For the induction step, suppose $\conf \ctxstepsto^m \conf''
  \ctxstepsto \conf'''$ and suppose the lemma holds for $m$.

  We show that it holds for $m + 1$, as follows.

  We are required to show that either:
  \begin{enumerate}
    \item there exist $\conf_c, i, j, \pi$ such that $\conf'
      \ctxstepsto^{i} \conf_c$ and $\pi(\conf''') \ctxstepsto^{j}
      \conf_c$ and $i \leq m + 1$ and $j \leq 1$, or
    \item there exists $k \leq m + 1$ such that $\conf' \ctxstepsto^k
      \error$, or there exists $k \leq 1$ such that $\conf'''
      \ctxstepsto^k \error$.
  \end{enumerate}

  From the induction hypothesis, we have that either:
  \begin{enumerate}
    \item there exist $\conf_c', i', j', \pi'$ such that $\conf'
      \ctxstepsto^{i'} \conf_c'$ and $\pi'(\conf'') \ctxstepsto^{j'}
      \conf_c'$ and $i' \leq m$ and $j' \leq 1$, or
    \item there exists $k' \leq m$ such that $\conf'
      \ctxstepsto^{k'} \error$, or there exists $k' \leq 1$ such that
      $\conf'' \ctxstepsto^{k'} \error$.
  \end{enumerate}

  We consider these two cases in turn:
  \begin{enumerate}
    \item There exist $\conf_c', i', j', \pi'$ such that $\conf'
      \ctxstepsto^{i'} \conf_c'$ and $\pi'(\conf'') \ctxstepsto^{j'}
      \conf_c'$ and $i' \leq m$ and $j' \leq 1$:

      We proceed by cases on $j'$:
      \begin{itemize}

      \item If $j' = 0$, then $\pi'(\conf'') = \conf_c'$.

        Since $\conf'' \ctxstepsto \conf'''$, we have that
        $\pi'(\conf'') \ctxstepsto \pi'(\conf''')$ by
        Lemma~\ref{lem:permutability} (Permutability).

        We can then choose $\conf_c = \pi'(\conf''')$ and $i = i' + 1$
        and $j = 0$ and $\pi = \pi'$.  The key is that $\conf'
        \ctxstepsto^{i'} \conf'_c = \pi'(\conf'') \ctxstepsto
        \pi'(\conf''')$ for a total of $i' + 1$ steps.
        
      \item If $j' = 1$:

        First, since $\pi'(\conf'') \ctxstepsto^{j'} \conf'_c$, then
        by Lemma~\ref{lem:permutability} (Permutability) we have that
        $\conf'' \ctxstepsto^{j'} \piprimeinv(\conf'_c)$.
        
        Then, by $\conf'' \ctxstepsto^{j'} \piprimeinv(\conf'_c)$ and
        $\conf'' \ctxstepsto \conf'''$ and
        Lemma~\ref{lem:strong-local-quasi-confluence}, one of the
        following two cases is true:
        \begin{enumerate}
        \item There exist $\conf_c''$ and $i''$ and $j''$ and $\pi''$
          such that $\piprimeinv(\conf'_c) \ctxstepsto^{i''}
          \conf_c''$ and $\pi''(\conf''') \ctxstepsto^{j''} \conf_c''$
          and $i'' \leq 1$ and $j'' \leq 1$.

          Since $\piprimeinv(\conf'_c) \ctxstepsto^{i''} \conf_c''$,
          by Lemma~\ref{lem:permutability} (Permutability) we have
          that $\conf'_c \ctxstepsto^{i''} \pi'(\conf_c'')$.

          So we also have $\conf' \ctxstepsto^{i'} \conf_c'
          \ctxstepsto^{i''} \pi'(\conf_c'')$.

          Since $\pi''(\conf''') \ctxstepsto^{j''} \conf_c''$, by
          Lemma~\ref{lem:permutability} (Permutability) we have that
          $\pi'(\pi''(\conf''')) \ctxstepsto^{j''} \pi'(\conf_c'')$.

          In summary, we pick $\conf_c = \pi'(\conf_c'')$ and $i = i' + i''$
          and $j = j''$ and $\pi = \pi'' \circ \pi'$, which is sufficient
          because $i = i' + i'' \leq m + 1$ and $j = j'' \leq 1$.

        \item $\piprimeinv(\conf'_c) \ctxstepsto \error$ or $\conf'''
          \ctxstepsto \error$.

          If $\conf''' \ctxstepsto \error$, then choosing $k = 1$
          satisfies the proof.

          Otherwise, $\piprimeinv(\conf'_c) \ctxstepsto \error$.
          Then, by Lemma~\ref{lem:permutability} we have that
          $\conf'_c \ctxstepsto \pi'(\error)$.  By
          Definition~\ref{def:permutation-configuration},
          $\pi'(\error) = \error$, and so $\conf'_c \ctxstepsto
          \error$. Therefore $\conf' \ctxstepsto^{i'} \conf'_c
          \ctxstepsto \error$.

          Hence $\conf' \ctxstepsto^{i'+1} \error$.

          Since $i' \leq m$, we have that $i' + 1 \leq m + 1$, and
          so choosing $k = i' + 1$ satisfies the proof.
            
        \end{enumerate}

      \end{itemize}

    \item There exists $k' \leq m$ such that $\conf' \ctxstepsto^{k'}
      \error$, or there exists $k' \leq 1$ such that $\conf''
      \ctxstepsto^{k'} \error$:

      If there exists $k' \leq m$ such that $\conf' \ctxstepsto^{k'}
      \error$, then choosing $k = k'$ satisfies the proof.

      Otherwise, there exists $k' \leq 1$ such that $\conf''
      \ctxstepsto^{k'} \error$.  We proceed by cases on $k'$:

      \begin{itemize}

      \item If $k' = 0$, then $\conf'' = \error$.

        Hence this case is not possible, since $\conf'' \ctxstepsto
        \conf'''$ and $\error$ cannot step.

      \item If $k' = 1$:

        From $\conf'' \ctxstepsto \conf'''$ and $\conf''
        \ctxstepsto^{k'} \error$ and
        Lemma~\ref{lem:strong-local-quasi-confluence}, one of the
        following two cases is true:

        \begin{enumerate}
        \item There exist $\conf_c''$ and $i''$ and $j''$ and $\pi''$
          such that $\error \ctxstepsto^{i''} \conf_c''$ and
          $\pi''(\conf''') \ctxstepsto^{j''} \conf_c''$ and $i'' \leq
          1$ and $j'' \leq 1$.

          Since $\error$ cannot step, $i'' = 0$ and $\conf''_c =
          \error$.

          By Definition~\ref{def:permutation-configuration},
          $\pi''(\conf''') = \conf'''$.

          Hence $\conf''' \ctxstepsto^{j''} \error$.

          \lk{This is the one place that we need to allow $k$ to be
            $\leq$ 1 instead of exactly 1.}

          Since $j'' \leq 1$, choosing $k = j''$ satisfies the proof.

        \item $\error \ctxstepsto \error$ or $\conf''' \ctxstepsto
          \error$.

          Since $\error$ cannot step, $\conf''' \ctxstepsto \error$.

          Hence choosing $k = 1$ satisfies the proof.

        \end{enumerate}

      \end{itemize}

  \end{enumerate}

\end{proof}
