\begin{proof}
  Suppose $\config{S}{\evalctxt{E_1}{e_1}} \ctxstepsto
  \config{S_1}{\evalctxt{E_1}{e'_1}}$ and
  $\config{S}{\evalctxt{E_2}{e_2}} \ctxstepsto
  \config{S_2}{\evalctxt{E_2}{e'_2}}$ and $\evalctxt{E_1}{e_1} =
  \evalctxt{E_2}{e_2}$.

  We are required to show that if $E_1 \neq E_2$, then there exist
  evaluation contexts $E'_1$ and $E'_2$ such that:
  \begin{itemize}
  \item $\evalctxt{E'_1}{e_1} = \evalctxt{E_2}{e'_2}$, and
  \item $\evalctxt{E'_2}{e_2} = \evalctxt{E_1}{e'_1}$, and
  \item $\evalctxt{E'_1}{e'_1} = \evalctxt{E'_2}{e'_2}$.
  \end{itemize}

  Let $e = \evalctxt{E_1}{e_1} = \evalctxt{E_2}{e_2}$.

  The proof is by induction on the structure of the expression $e$.

  Proceeding by cases on $e$:

  \begin{itemize}

  \item Cases $e = x$, $e = v$, $e = \app{e_a}{e_b}$, $e =
    \getexp{e_a}{e_b}$, and $e = \NEW$ are identical to their
    corresponding cases in the proof of
    Lemma~\ref{lem:lvars-locality}.

  \item Case $e = \putiexp{e_a}$:

    We know that $\putiexp{e_a} = \evalctxt{E_1}{e_1}$.

    From the grammar of evaluation contexts, then, we know that
    either:
    \begin{itemize}
    \item $\putiexp{e_a} = \evalctxt{E_1}{e_1} =
      \evalctxt{E_1}{\putiexp{e_a}}$, where $E_1 = [~]$, or
    \item $\putiexp{e_a} = \evalctxt{E_1}{e_1} =
      \putiexp{\evalctxt{E_{11}}{e_1}}$, where $\evalctxt{E_{11}}{e_1}
      = e_a$.
    \end{itemize}

    Similarly, we know that $\putiexp{e_a} = \evalctxt{E_2}{e_2}$.

    From the grammar of evaluation contexts, we know that either:
    \begin{itemize}
    \item $\putiexp{e_a} = \evalctxt{E_2}{e_2} =
      \evalctxt{E_2}{\putiexp{e_a}}$, where $E_2 = [~]$, or
    \item $\putiexp{e_a} = \evalctxt{E_2}{e_2} =
      \putiexp{\evalctxt{E_{21}}{e_2}}$, where $\evalctxt{E_{21}}{e_2}
      = e_a$.
    \end{itemize}

    However, if $E_1 = [~]$ or $E_2 = [~]$, then $\putiexp{e_a}$ must
    be $\putiexp{v}$ for some $v$, and $v$ cannot step individually,
    so the other of $E_1$ or $E_2$ must be $[~]$ as well, and so $E_1
    = E_2$.

    Therefore the only case that we have to consider (where $E_1 \neq
    E_2$) is the case in which $\evalctxt{E_1}{e_1} =
    \putiexp{\evalctxt{E_{11}}{e_1}}$, where $\evalctxt{E_{11}}{e_1} =
    e_a$, and $\putiexp{e_a} = \evalctxt{E_2}{e_2} =
    \putiexp{\evalctxt{E_{21}}{e_2}}$, where $\evalctxt{E_{21}}{e_2} =
    e_a$.

    So, we have $\evalctxt{E_{11}}{e_1} = e_a$ and
    $\evalctxt{E_{21}}{e_2} = e_a$.

    In this case, we know that $E_{11} \neq E_{21}$, because if
    $E_{11} = E_{21}$, we would have $e_1 = e_2$, which would mean
    that $E_1 = E_2$, a contradiction.

    So, since $E_{11} \neq E_{21}$, by IH we have that there exist
    evaluation contexts $E'_{11}$ and $E'_{21}$ such that:
    \begin{itemize}
    \item $\evalctxt{E'_{11}}{e_1} = \evalctxt{E_{21}}{e'_2}$, and
    \item $\evalctxt{E'_{21}}{e_2} = \evalctxt{E_{11}}{e'_1}$, and
    \item $\evalctxt{E'_{11}}{e'_1} = \evalctxt{E'_{21}}{e'_2}$.
    \end{itemize}

    Hence we can choose $E'_1 = \putiexp{E'_{11}}$ and $E'_2 =
    \putiexp{E'_{21}}$, which satisfy the criteria for $E'_1$ and
    $E'_2$.

  \item Case $e = \freeze{e_a}$: Similar to the case for
    $\putiexp{e_a}$.

  \item Case $e = \freezeafter{e_a}{e_b}{e_c}$: Similar to the case
    where $e = \app{e_a}{e_b}$.

  \item Case $e = \freezeafterfull{l}{Q}{\lam{x}{e_a}}{\setof{e_b,
      \dots}}{H}$:

    We know that $\freezeafterfull{l}{Q}{\lam{x}{e_a}}{\setof{e_b,
        \dots}}{H} = \evalctxt{E_1}{e_1}$.

    From the grammar of evaluation contexts, we know that either:
    \begin{itemize}
    \item $\freezeafterfull{l}{Q}{\lam{x}{e_a}}{\setof{e_b,
        \dots}}{H} = \evalctxt{E_1}{e_1} =$ \\
      $\evalctxt{E_1}{\freezeafterfull{l}{Q}{\lam{x}{e_a}}{\setof{e_b,
          \dots}}{H}}$, where $E_1 = [~]$, or
    \item $\freezeafterfull{l}{Q}{\lam{x}{e_a}}{\setof{e_b,
        \dots}}{H} = \evalctxt{E_1}{e_1} =$ \\
      $\freezeafterfull{l}{Q}{\lam{x}{e_a}}{\setof{e_{b_1}, \dots,
        \evalctxt{E_{11}}{e_1}, \dots, e_{b_n}}}{H}$, where
      $\evalctxt{E_{11}}{e_1} = e_{b_i}$.
    \end{itemize}

    Similarly, we know that
    $\freezeafterfull{l}{Q}{\lam{x}{e_a}}{\setof{e_b, \dots}}{H} =
    \evalctxt{E_2}{e_2}$.

    From the grammar of evaluation contexts, we know that either:
    \begin{itemize}
    \item $\freezeafterfull{l}{Q}{\lam{x}{e_a}}{\setof{e_b,
        \dots}}{H} = \evalctxt{E_2}{e_2} =$ \\
      $\evalctxt{E_2}{\freezeafterfull{l}{Q}{\lam{x}{e_a}}{\setof{e_b,
          \dots}}{H}}$, where $E_2 = [~]$, or
    \item $\freezeafterfull{l}{Q}{\lam{x}{e_a}}{\setof{e_b,
        \dots}}{H} = \evalctxt{E_2}{e_2} =$ \\
      $\freezeafterfull{l}{Q}{\lam{x}{e_a}}{\setof{e_{b_1}, \dots,
        \evalctxt{E_{21}}{e_2}, \dots, e_{b_n}}}{H}$, where
      $\evalctxt{E_{21}}{e_2} = e_{b_j}$.
    \end{itemize}

    However, if $E_1 = [~]$ or $E_2 = [~]$, then
    $\freezeafterfull{l}{Q}{\lam{x}{e_a}}{\setof{e_b, \dots}}{H}$ must
    be $\freezeafterfull{l}{Q}{\lam{x}{e_a}}{\setof{v, \dots}}{H}$ for
    some $\setof{v_1, \dots, v_n}$, and no $v_i$ can step
    individually, so the other of $E_1$ or $E_2$ must be $[~]$ as
    well, and so $E_1 = E_2$.

    Therefore the only case that we have to consider (where $E_1 \neq
    E_2$) is the case in which:
    \begin{itemize}
    \item $\freezeafterfull{l}{Q}{\lam{x}{e_a}}{\setof{e_b,
        \dots}}{H} = \evalctxt{E_1}{e_1} =$ \\
      $\freezeafterfull{l}{Q}{\lam{x}{e_a}}{\setof{e_{b_1}, \dots,
        \evalctxt{E_{11}}{e_1}, \dots, e_{b_n}}}{H}$, where
      $\evalctxt{E_{11}}{e_1} = e_{b_i}$, and
    \item $\freezeafterfull{l}{Q}{\lam{x}{e_a}}{\setof{e_b,
        \dots}}{H} = \evalctxt{E_2}{e_2} =$ \\
      $\freezeafterfull{l}{Q}{\lam{x}{e_a}}{\setof{e_{b_1}, \dots,
        \evalctxt{E_{21}}{e_2}, \dots, e_{b_n}}}{H}$, where
      $\evalctxt{E_{21}}{e_2} = e_{b_j}$.
    \end{itemize}

    Finally, we have two cases to consider:
    \begin{itemize}
    \item $e_{b_i} = e_{b_j}$: In this case we have $e_{b_i} =
      \evalctxt{E_{11}}{e_1} = \evalctxt{E_{21}}{e_2}$.

      We know that $E_{11} \neq E_{21}$, because if $E_{11} = E_{21}$,
      we would have $e_1 = e_2$, which would mean that $E_1 = E_2$, a
      contradiction.

      So, since $E_{11} \neq E_{21}$, by IH we have that there exist
      evaluation contexts $E'_{11}$ and $E'_{21}$ such that:
      \begin{itemize}
      \item $\evalctxt{E'_{11}}{e_1} = \evalctxt{E_{21}}{e'_2}$, and
      \item $\evalctxt{E'_{21}}{e_2} = \evalctxt{E_{11}}{e'_1}$, and
      \item $\evalctxt{E'_{11}}{e'_1} = \evalctxt{E'_{21}}{e'_2}$.
      \end{itemize}
      Hence we can choose
      \[E'_1 = \freezeafterfull{l}{Q}{\lam{x}{e_a}}{\setof{e_{b_1}, \dots,
          E'_{11}, \dots, e_{b_n}}}{H},\] and
      \[E'_2 = \freezeafterfull{l}{Q}{\lam{x}{e_a}}{\setof{e_{b_1}, \dots,
          E'_{21}, \dots, e_{b_n}}}{H},\] which satisfy the criteria
      for $E'_1$ and $E'_2$.

    \item $e_{b_i} \neq e_{b_j}$:
      In this case, we can choose
      \[E'_1 = \freezeafterfull{l}{Q}{\lam{x}{e_a}}{\setof{e_{b_1},
          \dots, E_{11}, \dots, \evalctxt{E_{21}}{e'_2}, \dots,
          e_{b_n}}}{H},\] and
      \[E'_2 = \freezeafterfull{l}{Q}{\lam{x}{e_a}}{\setof{e_{b_1},
          \dots, \evalctxt{E_{11}}{e'_1}, \dots, E_{21}, \dots,
          e_{b_n}}}{H},\] which satisfy the criteria for $E'_1$ and
      $E'_2$.
    \end{itemize}
  \end{itemize}
\end{proof}
