\begin{proof}
  Suppose that $\conf \ctxstepsto^n \conf'$ and $\conf \ctxstepsto^m
  \conf''$, where $1 \leq n$ and $1 \leq m$.

  We are required to show that either:
  \begin{enumerate}
  \item there exist $\conf_c, i, j, \pi$ such that $\conf'
    \ctxstepsto^i \conf_c$ and $\pi(\conf'') \ctxstepsto^j \conf_c$
    and $i \leq m$ and $j \leq n$, or
  \item there exists $k \leq m$ such that $\conf' \ctxstepsto^k
    \textup{\error}$, or there exists $k \leq n$ such that $\conf''
    \ctxstepsto^k \textup{\error}$.
  \end{enumerate}

  We proceed by induction on $n$.

  In the base case of $n = 1$, the result is immediate from
  Lemma~\ref{lem:strong-one-sided-quasi-confluence}.

  For the induction step, suppose $\conf \ctxstepsto^n \conf'
  \ctxstepsto \conf'''$ and suppose the lemma holds for $n$.

  We show that it holds for $n + 1$, as follows.

  From the induction hypothesis, we have that either:
  \begin{enumerate}
  \item there exist $\conf'_c, i', j', \pi'$ such that $\conf'
    \ctxstepsto^{i'} \conf'_c$ and $\pi'(\conf'') \ctxstepsto^{j'}
    \conf'_c$ and $i' \leq m$ and $j' \leq n$, or
  \item there exists $k' \leq m$ such that $\conf' \ctxstepsto^{k'}
    \error$, or there exists $k' \leq n$ such that $\conf''
    \ctxstepsto^{k'} \error$.
  \end{enumerate}

  We consider these two cases in turn:

  \begin{enumerate}
  \item There exist $\conf'_c, i', j', \pi'$ such that $\conf'
    \ctxstepsto^{i'} \conf'_c$ and $\pi'(\conf'') \ctxstepsto^{j'}
    \conf'_c$ and $i' \leq m$ and $j' \leq n$:

    We proceed by cases on $i'$:
    \begin{itemize}

    \item If $i' = 0$, then $\conf' = \conf_c'$.

      We can then choose $\conf_c = \conf'''$ and $i = 0$ and $j = j'
      + 1$ and $\pi = \pi'$.

      Since $\pi'(\conf'') \ctxstepsto^{j'} \conf'_c \ctxstepsto
      \conf'''$, and $j' + 1 \leq n + 1$ since $j' \leq n$, the case
      is satisfied.

    \item If $i' \geq 1$:

      From $\conf' \ctxstepsto \conf'''$ and $\conf' \ctxstepsto^{i'}
      \conf_c'$ and Lemma~\ref{lem:strong-one-sided-quasi-confluence},
      one of the following two cases is true:
      \begin{enumerate}
      \item There exist $\conf_c''$ and $i''$ and $j''$ and $\pi''$
        such that $\conf''' \ctxstepsto^{i''} \conf_c''$ and
        $\pi''(\conf_c') \ctxstepsto^{j''} \conf_c''$ and $i'' \leq
        i'$ and $j'' \leq 1$.

        Since $\pi'(\conf'') \ctxstepsto^{j'} \conf'_c$, by
        Lemma~\ref{lem:permutability} (Permutability) we have that
        $\pi''(\pi'(\conf'')) \ctxstepsto^{j'} \pi''(\conf'_c)$.

        So we also have $\pi''(\pi'(\conf'')) \ctxstepsto^{j'}
        \pi''(\conf'_c) \ctxstepsto^{j''} \conf_c''$.

        In summary, we pick $\conf_c = \conf_c''$ and $i = i''$ and $j =
        j' + j''$ and $\pi = \pi' \circ \pi''$, which is sufficient
        because $i = i'' \leq i' \leq m$ and $j = j' + j'' \leq n + 1$.

      \item There exists $k'' \leq i'$ such that $\conf'''
        \ctxstepsto^{k''} \error$, or there exists $k'' \leq 1$ such
        that $\conf'_c \ctxstepsto^{k''} \error$.

        If there exists $k'' \leq i'$ such that $\conf'''
        \ctxstepsto^{k''} \error$, then choosing $k = k''$ satisfies
        the proof, since $k'' \leq i' \leq m$.

        Otherwise, there exists $k'' \leq 1$ such
        that $\conf'_c \ctxstepsto^{k''} \error$.

        Hence by Lemma~\ref{lem:permutability} (Permutability), we
        have that $\piprimeinv(\conf'_c) \ctxstepsto^{k''}
        \piprimeinv(\error)$.

        By Definition~\ref{def:permutation-configuration},
        $\piprimeinv(\error) = \error$.

        Hence $\piprimeinv(\conf'_c) \ctxstepsto^{k''} \error$.

        Since $\pi'(\conf'') \ctxstepsto^{j'} \conf_c'$, by
        Lemma~\ref{lem:permutability} (Permutability), we have that
        $\conf'' \ctxstepsto^{j'} \piprimeinv(\conf_c')$.

        Therefore, $\conf'' \ctxstepsto^{j'} \piprimeinv(\conf_c')
        \ctxstepsto^{k''} \error$.

        Hence $\conf'' \ctxstepsto^{j' + k''} \error$.

        Since $j' \leq n$ and $k'' \leq 1$, $j' + k'' \leq n + 1$.

        Hence choosing $k = j' + k''$ satisfies the proof.

      \end{enumerate}
    \end{itemize}

  \item There exists $k' \leq m$ such that $\conf' \ctxstepsto^{k'}
    \error$, or there exists $k' \leq n$ such that $\conf''
    \ctxstepsto^{k'} \error$:

    If there exists $k' \leq n$ such that $\conf'' \ctxstepsto^{k'}
    \error$, then choosing $k = k'$ satisfies the proof.

    Otherwise, there exists $k' \leq m$ such that $\conf'
    \ctxstepsto^{k'} \error$.

    We proceed by cases on $k'$:

    \begin{itemize}

    \item If $k' = 0$, then $\conf' = \error$.

      Hence this case is not possible, since $\conf' \ctxstepsto
      \conf'''$ and $\error$ cannot step.

    \item If $k' \geq 1$:

      From $\conf' \ctxstepsto \conf'''$ and $\conf' \ctxstepsto^{k'}
      \error$ and Lemma~\ref{lem:strong-one-sided-quasi-confluence},
      one of the following two cases is true:

      \begin{enumerate}
      \item There exist $\conf''_c$ and $i''$ and $j''$ and $\pi''$
        such that $\conf''' \ctxstepsto^{i''} \conf''_c$ and
        $\pi''(\error) \ctxstepsto^{j''} \conf''_c$ and $i'' \leq
        k'$ and $j'' \leq 1$.

        By Definition~\ref{def:permutation-configuration},
        $\pi''(\error) = \error$.

        Hence $\error \ctxstepsto^{j''} \conf''_c$.

        Since $\error$ cannot step, $j'' = 0$ and $\conf''_c =
        \error$.

        Hence $\conf''' \ctxstepsto^{i''} \error$.

        Since $i'' \leq k' \leq m$, choosing $k = i''$ satisfies the
        proof.

      \item There exists $k'' \leq k'$ such that $\conf'''
        \ctxstepsto^{k''} \error$, or there exists $k'' \leq 1$ such
        that $\error \ctxstepsto^{k''} \error$.

        Since $\error$ cannot step, there exists $k'' \leq k'$ such
        that $\conf''' \ctxstepsto^{k''} \error$.

        Since $k'' \leq k' \leq m$, choosing $k = k''$ satisfies the
        proof.
      \end{enumerate}
    \end{itemize}
  \end{enumerate}

\end{proof}
