\begin{proof}
  Suppose $\config{S}{\evalctxt{E_1}{e_1}} \ctxstepsto \config{S_1}{\evalctxt{E_1}{e'_1}}$ and
  $\config{S}{\evalctxt{E_2}{e_2}} \ctxstepsto
  \config{S_2}{\evalctxt{E_2}{e'_2}}$ and $\evalctxt{E_1}{e_1} =
  \evalctxt{E_2}{e_2}$.

  We are required to show that if $E_1 \neq E_2$, then there exist
  evaluation contexts $E'_1$ and $E'_2$ such that:
  \begin{itemize}
  \item $\evalctxt{E'_1}{e_1} = \evalctxt{E_2}{e'_2}$, and
  \item $\evalctxt{E'_2}{e_2} = \evalctxt{E_1}{e'_1}$, and
  \item $\evalctxt{E'_1}{e'_1} = \evalctxt{E'_2}{e'_2}$.
  \end{itemize}

  Let $e = \evalctxt{E_1}{e_1} = \evalctxt{E_2}{e_2}$.  The proof is
  by induction on the structure of the expression $e$.  Proceeding by
  cases:

  \begin{itemize}

    \item Case $x$: In this case, the only possible context for $E_1$
      and $E_2$ is the empty context $[~]$.  Therefore $E_1 = E_2$,
      and so the case holds vacuously.

    \item Case $v$: Similar to the case for $x$.

    \item Case $\app{e_a}{e_b}$:

      We know that $\evalctxt{E_1}{e_1} = e$.  From the grammar of
      evaluation contexts, we know that either:
      \begin{itemize}
        \item $e = \evalctxt{E_1}{e_1} = \app{\evalctxt{E_a}{e_1}}{e_b}$, where $\evalctxt{E_a}{e_1} = e_a$, or
        \item $e = \evalctxt{E_1}{e_1} = \app{e_a}{\evalctxt{E_a}{e_1}}$, where $\evalctxt{E_a}{e_1} = e_b$.
      \end{itemize}

      Similarly, we know that $\evalctxt{E_2}{e_2} = e$.  From the grammar of
      evaluation contexts, we know that either:
      \begin{itemize}
        \item $e = \evalctxt{E_2}{e_2} = \app{\evalctxt{E_b}{e_2}}{e_b}$, where $\evalctxt{E_b}{e_2} = e_a$, or
        \item $e = \evalctxt{E_2}{e_2} = \app{e_a}{\evalctxt{E_b}{e_2}}$, where $\evalctxt{E_b}{e_2} = e_b$.
      \end{itemize}

      This gives us four sub-cases to consider:

      \TODO{Finish this.}

    \item Case $\getexp{e_a}{e_b}$: Similar to the case for $\app{e_a}{e_b}$.

    \item Case $\putexp{e_a}{e_b}$: Similar to the case for $\app{e_a}{e_b}$.

    \item Case $\NEW$: Similar to the case for $x$.
  \end{itemize}
\end{proof}
