\begin{proof}
  We proceed by induction on $m$.  In the base case of $m = 1$, the
  result is immediate from
  Lemma~\ref{lem:strong-local-quasi-confluence}, with $k = 1$.

  For the induction step, suppose $\conf \parstepsto^m \conf''
  \parstepsto \conf'''$ and suppose the lemma holds for $m$.

  We show that it holds for $m + 1$, as follows.

  We are required to show that either:
  \begin{enumerate}
    \item there exist $\conf_c, i,
      j$ such that $\conf' \parstepsto^{i} \conf_c$ and $\conf'''
      \parstepsto^{j} \conf_c$ and $i \leq m + 1$ and $j \leq 1$, or
    \item there exists $k \leq m + 1$ such that $\conf' \parstepsto^k
      \error$, or there exists $k \leq 1$ such that $\conf'''
      \parstepsto^k \error$.
  \end{enumerate}

  From the induction hypothesis, we have that either:
  \begin{enumerate}
    \item there exist $\conf_c', i',
      j'$ such that $\conf' \parstepsto^{i'} \conf_c'$ and $\conf''
      \parstepsto^{j'} \conf_c'$ and $i' \leq m$ and $j' \leq 1$, or
    \item there exists $k' \leq m$ such that $\conf'
      \parstepsto^{k'} \error$, or there exists $k' \leq 1$ such that
      $\conf'' \parstepsto^{k'} \error$.
  \end{enumerate}

  We consider these two cases in turn:
  \begin{enumerate}
    \item There exist $\conf_c', i',
      j'$ such that $\conf' \parstepsto^{i'} \conf_c'$ and $\conf''
      \parstepsto^{j'} \conf_c'$ and $i' \leq m$ and $j' \leq 1$:

      \lk{This gets very hairy.  I could spell things out in more
        detail, but it's MUCH better explained with a drawing, which
        I'm happy to do later. :)}

      We proceed by cases on $j'$:
      \begin{itemize}

      \item If $j' = 0$, then $\conf'' = \conf_c'$.  We can then
        choose $\conf_c = \conf'''$ and $i = i' + 1$ and $j = 0$.

        
      \item If $j' = 1$:
        
        From $\conf'' \parstepsto \conf'''$ and $\conf''
        \parstepsto^{j'} \conf_c'$ and
        Lemma~\ref{lem:strong-local-quasi-confluence}, one of the
        following two cases is true:
        \begin{enumerate}
        \item There exist $\conf_c''$ and $i''$ and $j''$ such that
          $\conf'_c \parstepsto^{i''} \conf_c''$ and $\conf'''
          \parstepsto^{j''} \conf_c''$ and $i'' \leq 1$ and $j''
          \leq 1$.  So we also have $\conf' \parstepsto^{i'}
          \conf_c' \parstepsto^{i''} \conf_c''$.  In summary, we
          pick $\conf_c = \conf_c''$ and $i = i' + i''$ and $j =
          j''$, which is sufficient because $i = i' + i'' \leq m +
          1$ and $j = j'' \leq 1$.
        \item $\conf''' \parstepsto \error$ or $\conf'_c \parstepsto
          \error$.

          If $\conf''' \parstepsto \error$, then choosing $k = 1$
          satisfies the proof.

          Otherwise, $\conf'_c \parstepsto \error$, therefore $\conf'
          \parstepsto^{i'} \conf'_c \parstepsto \error$.

          Hence $\conf' \parstepsto^{i'+1} \error$.

          Since $i' \leq m$, we have that $i' + 1 \leq m + 1$, and
          so choosing $k = i' + 1$ satisfies the proof.
            
        \end{enumerate}

      \end{itemize}

    \item There exists $k' \leq m$ such that $\conf' \parstepsto^{k'}
      \error$, or there exists $k' \leq 1$ such that $\conf''
      \parstepsto^{k'} \error$:

      If there exists $k' \leq m$ such that $\conf' \parstepsto^{k'}
      \error$, then choosing $k = k'$ satisfies the proof.

      Otherwise, there exists $k' \leq 1$ such that $\conf''
      \parstepsto^{k'} \error$.  We proceed by cases on $k'$:

      \begin{itemize}

      \item If $k' = 0$, then $\conf'' = \error$.

        Hence this case is not possible, since $\conf'' \parstepsto
        \conf'''$ and $\error$ cannot step.

      \item If $k' = 1$:

        From $\conf'' \parstepsto \conf'''$ and $\conf''
        \parstepsto^{k'} \error$ and
        Lemma~\ref{lem:strong-local-quasi-confluence}, one of the
        following two cases is true:

        \begin{enumerate}
        \item There exist $\conf_c''$ and $i''$ and $j''$ such that
          $\error \parstepsto^{i''} \conf_c''$ and $\conf'''
          \parstepsto^{j''} \conf_c''$ and $i'' \leq 1$ and $j''
          \leq 1$.

          Since $\error$ cannot step, $i'' = 0$ and $\conf''_c =
          \error$.

          Hence $\conf''' \parstepsto^{j''} \error$.

          \lk{This is the one place that we need to allow $k$ to be
            $\leq$ 1 instead of exactly 1.}

          Since $j'' \leq 1$, choosing $k = j''$ satisfies the proof.

        \item $\error \parstepsto \error$ or $\conf''' \parstepsto
          \error$.

          Since $\error$ cannot step, $\conf''' \parstepsto \error$.

          Hence choosing $k = 1$ satisfies the proof.

        \end{enumerate}

      \end{itemize}

  \end{enumerate}

\end{proof}
