\begin{proof}
  We proceed by induction on $n$.  In the base case of $n = 1$, the
  result is immediate from Lemma~\ref{lem:strong-one-sided-quasi-confluence}.

  For the induction step, suppose $\conf \parstepsto^n \conf'
  \parstepsto \conf'''$ and suppose the lemma holds for $n$.

  We show that it holds for $n + 1$, as follows.

  We are required to show that either:
  \begin{enumerate}
  \item there exist $\conf_c, i, j$ such that $\conf''' \parstepsto^i
    \conf_c$ and $\conf'' \parstepsto^j \conf_c$ and $i \leq m$ and $j
    \leq n + 1$, or
  \item there exists $k \leq m$ such that $\conf''' \parstepsto^k
    \error$, or there exists $k \leq n + 1$ such that $\conf''
    \parstepsto^k \error$.
  \end{enumerate}

  From the induction hypothesis, we have that either:
  \begin{enumerate}
  \item there exist $\conf'_c, i', j'$ such that $\conf'
    \parstepsto^{i'} \conf'_c$ and $\conf'' \parstepsto^{j'} \conf'_c$
    and $i' \leq m$ and $j' \leq n$, or
  \item there exists $k' \leq m$ such that $\conf' \parstepsto^{k'}
    \error$, or there exists $k' \leq n$ such that $\conf''
    \parstepsto^{k'} \error$.
  \end{enumerate}

  We consider these two cases in turn:

  \begin{enumerate}
  \item There exist $\conf'_c, i', j'$ such that $\conf'
    \parstepsto^{i'} \conf'_c$ and $\conf'' \parstepsto^{j'} \conf'_c$
    and $i' \leq m$ and $j' \leq n$:

    We proceed by cases on $i'$:
    \begin{itemize}

    \item If $i' = 0$, then $\conf' = \conf_c'$.  We can then choose
      $\conf_c = \conf'''$ and $i = 0$ and $j = j' + 1$.

    \item If $i' \geq 1$:

      From $\conf' \parstepsto \conf'''$ and $\conf' \parstepsto^{i'}
      \conf_c'$ and Lemma~\ref{lem:strong-one-sided-quasi-confluence},
      one of the following two cases is true:
      \begin{enumerate}
        \item There exist $\conf_c''$ and $i''$ and $j''$ such that
          $\conf''' \parstepsto^{i''} \conf_c''$ and $\conf_c'
          \parstepsto^{j''} \conf_c''$ and $i'' \leq i'$ and $j'' \leq
          1$.  So we also have $\conf'' \parstepsto^{j'} \conf_c'
          \parstepsto^{j''} \conf_c''$.  In summary, we pick $\conf_c
          = \conf_c''$ and $i = i''$ and $j = j' + j''$, which is
          sufficient because $i = i'' \leq i' \leq m$ and $j = j' +
          j'' \leq n + 1$.
        \item There exists $k'' \leq i'$ such that $\conf'''
          \parstepsto^{k''} \error$, or there exists $k'' \leq 1$ such
          that $\conf'_c \parstepsto^{k''} \error$.

          If there exists $k'' \leq i'$ such that $\conf'''
          \parstepsto^{k''} \error$, then choosing $k = k''$ satisfies
          the proof, since $k'' \leq i' \leq m$.

          Otherwise, there exists $k'' \leq 1$ such
          that $\conf'_c \parstepsto^{k''} \error$.

          Therefore, $\conf'' \parstepsto^{j'} \conf_c'
          \parstepsto^{k''} \error$.

          Hence $\conf'' \parstepsto^{j' + k''} \error$.

          Since $j' \leq n$ and $k'' \leq 1$, $j' + k'' \leq n + 1$.

          Hence choosing $k = j' + k''$ satisfies the proof.

      \end{enumerate}
    \end{itemize}

  \item There exists $k' \leq m$ such that $\conf' \parstepsto^{k'}
    \error$, or there exists $k' \leq n$ such that $\conf''
    \parstepsto^{k'} \error$:

    If there exists $k' \leq n$ such that $\conf'' \parstepsto^{k'}
    \error$, then choosing $k = k'$ satisfies the proof.

    Otherwise, there exists $k' \leq m$ such that $\conf'
    \parstepsto^{k'} \error$.  We proceed by cases on $k'$:

    \begin{itemize}

    \item If $k' = 0$, then $\conf' = \error$.

      Hence this case is not possible, since $\conf' \parstepsto
      \conf'''$ and $\error$ cannot step.

    \item If $k' \geq 1$:

      From $\conf' \parstepsto \conf'''$ and $\conf' \parstepsto^{k'}
      \error$ and Lemma~\ref{lem:strong-one-sided-quasi-confluence},
      one of the following two cases is true:

      \begin{enumerate}
        \item There exist $\conf''_c$ and $i''$ and $j''$ such that
          $\conf''' \parstepsto^{i''} \conf''_c$ and $\error
          \parstepsto^{j''} \conf''_c$ and $i'' \leq k'$ and $j'' \leq
          1$.

          Since $\error$ cannot step, $j'' = 0$ and $\conf''_c =
          \error$.

          Hence $\conf''' \parstepsto^{i''} \error$.

          Since $i'' \leq k' \leq m$, choosing $k = i''$ satisfies the
          proof.

        \item There exists $k'' \leq k'$ such that $\conf'''
          \parstepsto^{k''} \error$, or there exists $k'' \leq 1$ such
          that $\error \parstepsto^{k''} \error$.

          Since $\error$ cannot step, there exists $k'' \leq k'$ such
          that $\conf''' \parstepsto^{k''} \error$.

          Since $k'' \leq k' \leq m$, choosing $k = k''$ satisfies the
          proof.
      \end{enumerate}
    \end{itemize}
  \end{enumerate}

\end{proof}
