\begin{proof}
  By induction on the derivation of $\conf \parstepsto \conf_a$, by
  cases on the last rule in the derivation.

  \begin{itemize}
    \item {\sc E-Eval-Ctxt}: \TODO{Figure out what to do here.}

    \item {\sc E-Beta}: $\conf = \config{S}{\app{(\lam{x}{e})}{v}}$,
      and $\conf_a = \config{S}{\subst{e}{x}{v}}$.

      Given:
      \begin{itemize}
      \item $\config{S}{\app{(\lam{x}{e})}{v}} \parstepsto
        \config{S}{\subst{e}{x}{v}}$, and
      \item $\config{S}{\app{(\lam{x}{e})}{v}} \parstepsto \conf_b$.
      \end{itemize}

      To show: There exist $\conf_c, i, j$ such that

      $\config{S}{\subst{e}{x}{v}} \parstepsto^i \conf_c$ and $\conf_b
      \parstepsto^j \conf_c$ and $i \leq 1$ and $j \leq 1$.

      By inspection of the operational semantics, $\conf_b =
      \config{S}{\subst{e}{x}{v}}$.

      Choose $\conf_c = \config{S}{\subst{e}{x}{v}}$, $i = 0$ and $j =
      0$.

      Then $\config{S}{\subst{e}{x}{v}} = \conf_c$ and $\conf_b =
      \conf_c$, as required.

    \item {\sc E-New}: $\conf = \config{S}{\NEW}$, and $\conf_a =
      \config{\extS{S}{l}{\bot}{\frozenfalse}}{l}$.

      Given:
      \begin{itemize}
      \item $\config{S}{\NEW} \parstepsto
        \config{\extS{S}{l}{\bot}{\frozenfalse}}{l}$, and
      \item $\config{S}{\NEW} \parstepsto \conf_b$.
      \end{itemize}

      To show: There exist $\conf_c, i, j$ such that

      $\config{\extS{S}{l}{\bot}{\frozenfalse}}{l} \parstepsto^i
      \conf_c$ and $\conf_b \parstepsto^j \conf_c$ and $i \leq 1$ and
      $j \leq 1$.

      By inspection of the operational semantics, $\conf_b =
      \config{\extS{S}{l'}{\bot}{\frozenfalse}}{l'}$.

      From the side condition of {\sc E-New}, $l \notin S$.

      Therefore, in $\config{\extS{S}{l'}{\bot}{\frozenfalse}}{l'}$,
      we can $\alpha$-rename $l'$ to $l$, resulting in
      $\config{\extS{S}{l}{\bot}{\frozenfalse}}{l}$.

      Choose $\conf_c = \config{\extS{S}{l}{\bot}{\frozenfalse}}{l}$,
      $i = 0$ and $j = 0$.

      Then $\config{S}{\subst{e}{x}{v}} = \conf_c$ and $\conf_b =
      \conf_c$, as required.

    \item {\sc E-Put}: $\conf = \config{S}{\putexp{l}{d_2}}$, and
      $\conf_a = \config{\extSRaw{S}{l}{p_2}}{\unit}$.

      Given:
      \begin{itemize}
      \item $\config{S}{\putexp{l}{d_2}} \parstepsto
        \config{\extSRaw{S}{l}{p_2}}{\unit}$, and
      \item $\config{S}{\putexp{l}{d_2}} \parstepsto \conf_b$.
      \end{itemize}

      To show: There exist $\conf_c, i, j$ such that

      $\config{\extSRaw{S}{l}{p_2}}{\unit} \parstepsto^i \conf_c$ and
      $\conf_b \parstepsto^j \conf_c$ and $i \leq 1$ and $j \leq 1$.

      By inspection of the operational semantics, $\conf_b =
      \config{\extSRaw{S}{l}{p_2}}{\unit}$.

      Choose $\conf_c = \config{\extSRaw{S}{l}{p_2}}{\unit}$, $i = 0$
      and $j = 0$.

      Then $\config{\extSRaw{S}{l}{p_2}}{\unit} = \conf_c$ and $\conf_b
      = \conf_c$, as required.

    \item {\sc E-Put-Err}: $\conf = \config{S}{\putexp{l}{d_2}}$, and
      $\conf_a = \error$.

      Given:
      \begin{itemize}
      \item $\config{S}{\putexp{l}{d_2}} \parstepsto \error$, and
      \item $\config{S}{\putexp{l}{d_2}} \parstepsto \conf_b$.
      \end{itemize}

      To show: There exist $\conf_c, i, j$ such that

      $\error \parstepsto^i \conf_c$ and $\conf_b \parstepsto^j
      \conf_c$ and $i \leq 1$ and $j \leq 1$.

      By inspection of the operational semantics, $\conf_b = \error$.

      Choose $\conf_c = \error$, $i = 0$ and $j = 0$.

      Then $\error = \conf_c$ and $\conf_b = \conf_c$, as required.

    \item {\sc E-Get}: $\conf = \config{S}{\getexp{l}{P}}$, and
      $\conf_a = \config{S}{p_2}$.

      Given:
      \begin{itemize}
      \item $\config{S}{\getexp{l}{P}} \parstepsto \config{S}{p_2}$,
        and
      \item $\config{S}{\getexp{l}{P}} \parstepsto \conf_b$.
      \end{itemize}

      To show: There exist $\conf_c, i, j$ such that

      $\config{S}{p_2} \parstepsto^i \conf_c$ and $\conf_b
      \parstepsto^j \conf_c$ and $i \leq 1$ and $j \leq 1$.

      By inspection of the operational semantics, $\conf_b =
      \config{S}{p_2}$.

      Choose $\conf_c = \config{S}{p_2}$, $i = 0$ and $j = 0$.

      Then $\config{S}{p_2} = \conf_c$ and $\conf_b = \conf_c$, as
      required.

    \item {\sc E-Freeze-Init}: $\conf =
      \config{S}{\freezeafter{l}{Q}{\lam{x}{e}}}$, and $\conf_a =
      \config{S}{\freezeafterfull{l}{Q}{\lam{x}{e}}{\setof{}}{\setof{}}}$.

      Given:
      \begin{itemize}
      \item $\config{S}{\freezeafter{l}{Q}{\lam{x}{e}}} \parstepsto
        \config{S}{\freezeafterfull{l}{Q}{\lam{x}{e}}{\setof{}}{\setof{}}}$,
        and
      \item $\config{S}{\freezeafter{l}{Q}{\lam{x}{e}}} \parstepsto
        \conf_b$.
      \end{itemize}

      To show: There exist $\conf_c, i, j$ such that

      $\config{S}{\freezeafterfull{l}{Q}{\lam{x}{e}}{\setof{}}{\setof{}}}
      \parstepsto^i \conf_c$ and $\conf_b \parstepsto^j \conf_c$ and
      $i \leq 1$ and $j \leq 1$.

      By inspection of the operational semantics, $\conf_b =
      \config{S}{\freezeafterfull{l}{Q}{\lam{x}{e}}{\setof{}}{\setof{}}}$.

      Choose $\conf_c =
      \config{S}{\freezeafterfull{l}{Q}{\lam{x}{e}}{\setof{}}{\setof{}}}$,
      $i = 0$ and $j = 0$.

      Then
      $\config{S}{\freezeafterfull{l}{Q}{\lam{x}{e}}{\setof{}}{\setof{}}}
      = \conf_c$ and $\conf_b = \conf_c$, as required.

    \item {\sc E-Spawn-Handler}: $\conf =
      \config{S}{\freezeafterfull{l}{Q}{\lam{x}{e_0}}{\setof{e,
            \dots}}{H}}$, and

      $\conf_a =
      \config{S}{\freezeafterfull{l}{Q}{\lam{x}{e_0}}{\setof{\subst{e_0}{x}{d_2},
            e, \dots}} {\{d_2\}\cup H}}$.

      Given:
      \begin{itemize}
      \item $\config{S}{\freezeafterfull{l}{Q}{\lam{x}{e_0}}{\setof{e,
            \dots}}{H}} \parstepsto \\
        \config{S}{\freezeafterfull{l}{Q}{\lam{x}{e_0}}{\setof{\subst{e_0}{x}{d_2},
              e, \dots}} {\{d_2\}\cup H}}$, and
      \item $\config{S}{\freezeafterfull{l}{Q}{\lam{x}{e_0}}{\setof{e,
            \dots}}{H}} \parstepsto \conf_b$.
      \end{itemize}

      To show: There exist $\conf_c, i, j$ such that

      $\config{S}{\freezeafterfull{l}{Q}{\lam{x}{e_0}}{\setof{\subst{e_0}{x}{d_2},
            e, \dots}} {\{d_2\}\cup H}} \parstepsto^i \conf_c$ and
      $\conf_b \parstepsto^j \conf_c$ and $i \leq 1$ and $j \leq 1$.

      \lk{This time, we could actually get different results on the
        two sides of the diamond because we could choose a different
        $d_2$, or we could run a different expression in $\setof{e,
          \dots}$.}

      By inspection of the operational semantics, one of the following
      possibilities must hold:
      \begin{itemize}
      \item $\conf \parstepsto \conf_b$ by {\sc E-Spawn-Handler}:

        Hence $\conf_b =
        \config{S}{\freezeafterfull{l}{Q}{\lam{x}{e_0}}{\setof{\subst{e_0}{x}{d'_2},
              e, \dots}} {\{d'_2\}\cup H}}$.

        Here, there are two subcases:
        \begin{itemize}
        \item $d'_2 \neq d_2$:

          Choose: \\ 

          $\conf_c = \config{S}{\freezeafterfull{l}{Q}{\lam{x}{e_0}}{\setof{\subst{e_0}{x}{d_2},
                \subst{e_0}{x}{d'_2}, e, \dots}} {\{d_2, d'_2\}\cup H}}$, \\
          $i = 1$ and $j = 1$.

          To show:
          \begin{enumerate}
          \item $\conf_a \parstepsto \conf_c$, where \\
            $\conf_a = \config{S}{\freezeafterfull{l}{Q}{\lam{x}{e_0}}{\setof{\subst{e_0}{x}{d_2},
                e, \dots}} {\{d_2\}\cup H}}$ and \\
            $\conf_c = \config{S}{\freezeafterfull{l}{Q}{\lam{x}{e_0}}{\setof{\subst{e_0}{x}{d_2},
                  \subst{e_0}{x}{d'_2}, e, \dots}} {\{d_2, d'_2\}\cup H}}$.

            The proof is as follows:

            From the premises of {\sc E-Spawn-Handler}, \\
            $S(l) = \state{d_1}{\status_1}$ and
            $d'_2 \userleq d_1$ and 
            $d'_2 \notin H$ and
            $d'_2 \in Q$.

            Therefore, by {\sc E-Spawn-Handler}, \\
            $\config{S}{\freezeafterfull{l}{Q}{\lam{x}{e_0}}{\setof{\subst{e_0}{x}{d_2},
                e, \dots}} {\{d_2\}\cup H}} \parstepsto \\
            \config{S}{\freezeafterfull{l}{Q}{\lam{x}{e_0}}{\setof{\subst{e_0}{x}{d'_2}, \subst{e_0}{x}{d_2},
                  e, \dots}} \setof{d'_2} \cup {\{d_2\}\cup H}}$, \\
            which is equivalent to \\

            $\config{S}{\freezeafterfull{l}{Q}{\lam{x}{e_0}}{\setof{\subst{e_0}{x}{d_2},
                  \subst{e_0}{x}{d'_2}, e, \dots}} {\{d_2, d'_2\}\cup
                H}}$.

            Hence $\conf_a \parstepsto \conf_c$.

          \item $\conf_b \parstepsto \conf_c$, where \\
            $\conf_b = \config{S}{\freezeafterfull{l}{Q}{\lam{x}{e_0}}{\setof{\subst{e_0}{x}{d'_2},
                e, \dots}} {\{d'_2\}\cup H}}$, and \\
            $\conf_c = \config{S}{\freezeafterfull{l}{Q}{\lam{x}{e_0}}{\setof{\subst{e_0}{x}{d_2},
                  \subst{e_0}{x}{d'_2}, e, \dots}} {\{d_2, d'_2\}\cup H}}$.

            The proof is as follows:

            From the premises of {\sc E-Spawn-Handler}, \\
            $S(l) = \state{d_1}{\status_1}$ and
            $d_2 \userleq d_1$ and 
            $d_2 \notin H$ and
            $d_2 \in Q$.

            Therefore, by {\sc E-Spawn-Handler}, \\
            $\config{S}{\freezeafterfull{l}{Q}{\lam{x}{e_0}}{\setof{\subst{e_0}{x}{d'_2},
                  e, \dots}} {\{d'_2\}\cup H}} \parstepsto \\
            \config{S}{\freezeafterfull{l}{Q}{\lam{x}{e_0}}{\setof{\subst{e_0}{x}{d_2}, \subst{e_0}{x}{d'_2},
                  e, \dots}} \setof{d_2} \cup {\{d'_2\}\cup H}}$, \\
            which is equivalent to \\

            $\config{S}{\freezeafterfull{l}{Q}{\lam{x}{e_0}}{\setof{\subst{e_0}{x}{d_2},
                  \subst{e_0}{x}{d'_2}, e, \dots}} {\{d_2, d'_2\}\cup H}}$.

            Hence $\conf_b \parstepsto \conf_c$.
          \end{enumerate}

        \item $d'_2 = d_2$:

          Choose:
          $\conf_c = \config{S}{\freezeafterfull{l}{Q}{\lam{x}{e_0}}{\setof{\subst{e_0}{x}{d_2},
                e, \dots}} {\{d_2\}\cup H}}$, \\
          $i = 0$ and $j = 0$.

          Then
          $\config{S}{\freezeafterfull{l}{Q}{\lam{x}{e_0}}{\setof{\subst{e_0}{x}{d_2},
                e, \dots}} {\{d_2\}\cup H}} = \conf_c$ and $\conf_b =
          \conf_c$, as required.
        \end{itemize}

      \item $\conf \parstepsto \conf_b$ by {\sc E-Eval-Ctxt}:

        Hence $\conf_b =
        \config{S'}{\freezeafterfull{l}{Q}{\lam{x}{e_0}}{\setof{e',
              \dots}}{H}}$.

        \lk{Minor cheat here: the expression that could step could be
          \emph{any} expression in the set $\setof{e, \dots}$, not
          necessarily the first one.  I'm hoping it's enough to just
          write out this case.}

        Choose: \\
        $\conf_c = \config{S'}{\freezeafterfull{l}{Q}{\lam{x}{e_0}}{\setof{\subst{e_0}{x}{d_2},
              e', \dots}} {\{d_2\}\cup H}}$, \\
        $i = 1$ and $j = 1$.

        To show:
        \begin{enumerate}
        \item $\conf_a \parstepsto \conf_c$, where \\
          $\conf_a = \config{S}{\freezeafterfull{l}{Q}{\lam{x}{e_0}}{\setof{\subst{e_0}{x}{d_2},
              e, \dots}} {\{d_2\}\cup H}}$ and \\
          $\conf_c = \config{S'}{\freezeafterfull{l}{Q}{\lam{x}{e_0}}{\setof{\subst{e_0}{x}{d_2},
                e', \dots}} {\{d_2\}\cup H}}$.

          The proof is as follows:

          From the premise of {\sc E-Eval-Ctxt}, $\config{S}{e}
          \parstepsto \config{S'}{e'}$.

          From the definition of evaluation contexts, \\
          $\freezeafterfull{l}{Q}{\lam{x}{e_0}}{\setof{\subst{e_0}{x}{d_2},
                [~], \dots}} {\{d_2\}\cup H}$ \\
          is an evaluation context.

          Hence, by {\sc E-Eval-Ctxt}, \\
          $\config{S}{\freezeafterfull{l}{Q}{\lam{x}{e_0}}{\setof{\subst{e_0}{x}{d_2},
              e, \dots}} {\{d_2\}\cup H}} \parstepsto \\
          \config{S'}{\freezeafterfull{l}{Q}{\lam{x}{e_0}}{\setof{\subst{e_0}{x}{d_2},
                e', \dots}} {\{d_2\}\cup H}}$.
          
          Hence $\conf_a \parstepsto \conf_c$.

        \item $\conf_b \parstepsto \conf_c$, where \\
          $\conf_b = \config{S'}{\freezeafterfull{l}{Q}{\lam{x}{e_0}}{\setof{e',
              \dots}}{H}}$, and \\
          $\conf_c = \config{S'}{\freezeafterfull{l}{Q}{\lam{x}{e_0}}{\setof{\subst{e_0}{x}{d_2},
              e', \dots}} {\{d_2\}\cup H}}$.

          The proof is as follows:

          From the premises of {\sc E-Spawn-Handler}, \\
          $S(l) = \state{d_1}{\status_1}$ and
          $d_2 \userleq d_1$ and 
          $d_2 \notin H$ and
          $d_2 \in Q$.

          Hence, by {\sc E-Spawn-Handler}, \\
          $\config{S'}{\freezeafterfull{l}{Q}{\lam{x}{e_0}}{\setof{e',
              \dots}}{H}} \parstepsto \\
          \config{S'}{\freezeafterfull{l}{Q}{\lam{x}{e_0}}{\setof{\subst{e_0}{x}{d_2}, e',
                \dots}}{\{d_2\}\cup H}}$.

          Hence $\conf_b \parstepsto \conf_c$.
        \end{enumerate}

      \end{itemize}

    \item {\sc E-Freeze-Final}: $\conf =
      \config{S}{\freezeafterfull{l}{Q}{v}{\setof{v\dots}}{H}}$, and
      $\conf_a = \config{\extS{S}{l}{d_1}{\frozentrue}}{d_1}$.

      Given:
      \begin{itemize}
      \item $\config{S}{\freezeafterfull{l}{Q}{v}{\setof{v\dots}}{H}}
        \parstepsto \config{\extS{S}{l}{d_1}{\frozentrue}}{d_1}$, and
      \item $\config{S}{\freezeafterfull{l}{Q}{v}{\setof{v\dots}}{H}} \parstepsto \conf_b$.
      \end{itemize}

      To show: There exist $\conf_c, i, j$ such that

      $\config{\extS{S}{l}{d_1}{\frozentrue}}{d_1} \parstepsto^i
      \conf_c$ and $\conf_b \parstepsto^j \conf_c$ and $i \leq 1$ and
      $j \leq 1$.

      By inspection of the operational semantics, $\conf_b =
      \config{\extS{S}{l}{d_1}{\frozentrue}}{d_1}$.

      Choose $\conf_c = \config{\extS{S}{l}{d_1}{\frozentrue}}{d_1}$,
      $i = 0$ and $j = 0$.

      Then $\config{\extS{S}{l}{d_1}{\frozentrue}}{d_1} = \conf_c$ and
      $\conf_b = \conf_c$, as required.

    \item {\sc E-Freeze-Simple}: $\conf =
      \config{S}{\freeze{l}}$, and $\conf_a =
      \config{\extS{S}{l}{d_1}{\frozentrue}}{d_1}$.

      Given:
      \begin{itemize}
      \item $\config{S}{\freeze{l}} \parstepsto \config{\extS{S}{l}{d_1}{\frozentrue}}{d_1}$, and
      \item $\config{S}{\freeze{l}} \parstepsto \conf_b$.
      \end{itemize}

      To show: There exist $\conf_c, i, j$ such that
      $\config{\extS{S}{l}{d_1}{\frozentrue}}{d_1} \parstepsto^i
      \conf_c$ and $\conf_b \parstepsto^j \conf_c$ and $i \leq 1$ and
      $j \leq 1$.

      By inspection of the operational semantics, $\conf_b =
      \config{\extS{S}{l}{d_1}{\frozentrue}}{d_1}$.

      Choose $\conf_c = \config{\extS{S}{l}{d_1}{\frozentrue}}{d_1}$,
      $i = 0$ and $j = 0$.

      Then $\config{\extS{S}{l}{d_1}{\frozentrue}}{d_1} = \conf_c$ and
      $\conf_b = \conf_c$, as required.
  \end{itemize}
\end{proof}

